Make compilationLib output BVL and DataLang pretty print

compiler/backend/presLangLib.sig
@@ -1,0 +1,13 @@
+signature presLangLib =
+sig
+
+   include Abbrev
+
+   val data_to_strs : term (* names *) -> term (* prog *) -> string list
+   val bvl_to_strs : term (* names *) -> term (* prog *) -> string list
+
+   val print_strs : string list -> unit
+
+   val write_strs_to_file : string -> string list -> unit
+
+end
